src/Utilities.v
@@ -105,6 +105,8 @@ Definition equality_proof_irrelevance' {X:Type} {x y:X} (p q:x==y) :
   isaset X -> p==q.
 Proof. intros ? ? ? ? ? is. apply is. Defined.
 
+Definition funset X (Y:hSet) : hSet := hSetpair (X->Y) (impredfun 2 _ _ (pr2 Y)).
+
 Definition path_start {X} {x x':X} (p:x == x') := x.
 Definition path_end {X} {x x':X} (p:x == x') := x'.
 
